pcuic/theories/PCUICTyping.v
@@ -1381,7 +1381,7 @@ Proof.
          specialize (IH (existT _ (Σ, udecl) (existT _ X13 (existT _ _ (existT _ (typing_wf_local (Σ:=(Σ, udecl)) Hu)
                                                                            (existT _ _ (existT _ _ Hu))))))).
          simpl in IH. simpl. exists u. apply IH. constructor 1. simpl. lia.
-    + red in Xg. destruct Xg as [hctx [hr hpr]].
+    + red in Xg. destruct Xg as [hctx [hr [hpr hprr]]].
       split. 2: split.
       * eapply All_local_env_impl. 1: eassumption.
         intros Δ u T h. destruct T. all: simpl in h. all: simpl.
@@ -1417,31 +1417,34 @@ Proof.
               apply IH. constructor 1. simpl. lia.
         -- assumption.
         -- assumption.
-      * eapply All_impl. 1: eassumption.
-        intros rw [T onlhs onrhs onhead onelims].
-        exists T.
-        -- match type of IH with
-          | ?T -> _ =>
-            unshelve epose (y := _ : T)
-          end.
-          ++ exists (Σ, udecl). exists X13.
-              unshelve eexists _, _, _, _.
-              5: exact onlhs.
-              eapply typing_wf_local. eassumption.
-          ++ specialize (IH y). subst y. simpl in IH.
-              apply IH. constructor 1. simpl. lia.
-        -- match type of IH with
-          | ?T -> _ =>
-            unshelve epose (y := _ : T)
-          end.
-          ++ exists (Σ, udecl). exists X13.
-              unshelve eexists _, _, _, _.
-              5: exact onrhs.
-              eapply typing_wf_local. eassumption.
-          ++ specialize (IH y). subst y. simpl in IH.
-              apply IH. constructor 1. simpl. lia.
-        -- assumption.
-        -- assumption.
+      * split.
+        -- eapply All_impl. 1: exact hpr.
+           intros rw [T onlhs onrhs onhead onelims].
+           exists T.
+           ++ match type of IH with
+              | ?T -> _ =>
+                unshelve epose (y := _ : T)
+              end.
+              ** exists (Σ, udecl). exists X13.
+                  unshelve eexists _, _, _, _.
+                  5: exact onlhs.
+                  eapply typing_wf_local. eassumption.
+              ** specialize (IH y). subst y. simpl in IH.
+                  apply IH. constructor 1. simpl. lia.
+           ++ match type of IH with
+              | ?T -> _ =>
+                unshelve epose (y := _ : T)
+              end.
+              ** exists (Σ, udecl). exists X13.
+                  unshelve eexists _, _, _, _.
+                  5: exact onrhs.
+                  eapply typing_wf_local. eassumption.
+              ** specialize (IH y). subst y. simpl in IH.
+                  apply IH. constructor 1. simpl. lia.
+           ++ assumption.
+           ++ assumption.
+        -- eapply All_impl. 1: exact hprr.
+           cbn. intros rw h. auto.
 
   - assert (forall Γ (wfΓ : wf_local Σ Γ) t T (Hty : Σ ;;; Γ |- t : T),
                typing_size Hty < typing_size H ->
